Magic

examples/ghost_state.v
@@ -24,17 +24,37 @@ Proof. solve_inG. Qed.
 
 Context `{!heapGS Σ, !one_shotG Σ}.
 
+Lemma shoot_init : ⊢ |==> ∃ γ, own γ Pending.
+Proof.
+  iApply own_alloc.
+  done.
+Qed.
+
 Lemma shoot_upd γ : own γ Pending ==∗ own γ Shot.
 Proof.
   iApply own_update.
   apply shoot.
 Qed.
 
+Instance shot_persistent γ : Persistent (own γ Shot).
+Proof.
+  eapply own_core_persistent.
+  econstructor. done.
+Qed.
+
+Lemma shot_not_pending γ : own γ Shot -∗ own γ Pending -∗ False.
+Proof.
+  iIntros "H1 H2".
+  iPoseProof (own_valid_2 with "H1 H2") as "%H".
+  cbv in H.
+  done.
+Qed.
+
 End ghost_state.
 
 Section parallelism.
 
-Context `{!heapGS Σ, !one_shotG Σ}.
+Context `{!heapGS Σ, !one_shotG Σ, !spawnG Σ}.
 
 Definition flag_before_update : Z := 0.
 Definition flag_during_update : Z := 1.
@@ -43,34 +63,114 @@ Definition flag_after_update : Z := 2.
 Definition flag_invariant γ flag loc : iProp Σ :=
   ∃ f, flag ↦ #f ∗
     (loc ↦ #2 ∗ ⌜f = flag_before_update⌝ ∗ own γ Pending ∨
-     ⌜f = flag_during_update⌝ ∨
+     ⌜f = flag_during_update⌝ ∗ own γ Pending ∨
      loc ↦ #4 ∗ ⌜f = flag_after_update⌝ ∗ own γ Shot).
 
-Definition thread_body (flag loc : expr) : expr :=
-  rec: "thread_body" "_" :=
-    if: CAS flag #flag_before_update #flag_during_update
+Definition thread_body  : val :=
+  rec: "thread_body" "flag" "loc" :=
+    let: "pp" := CmpXchg "flag" #flag_before_update #flag_during_update in
+    let: "old_value" := Fst "pp" in
+    let: "did_exchange" := Snd "pp" in
+    if: "did_exchange"
       then
-        loc  <- ! loc + #2 ;;
-        flag <- #flag_after_update
-      else
-        if: !flag = #flag_during_update
-          then "thread_body" #()
-          else #().
+        "loc"  <- ! "loc" + #2 ;;
+        "flag" <- #flag_after_update
+      else if: "old_value" = #flag_during_update
+        then 
+          "thread_body" "flag" "loc"
+        else #().
 
 Lemma thread_helper γ flag loc N :
   inv N (flag_invariant γ flag loc)
   ⊢ WP (thread_body #flag #loc) {{ _, own γ Shot }}.
-Admitted.
+Proof.
+  iIntros "#Hinv".
+  iLöb as "IH".
+  wp_rec. wp_pures.
+  (* Focus on the CmpXchg, since it must be atomic *)
+  wp_bind (CmpXchg _ _ _).
+  (* Open the invariant *)
+  iInv "Hinv" as ">(%f&Hflag&Hcases)" "Hclose".
+  (* The invariant has a bunch of cases, let's analyze them *)
+  iDestruct "Hcases" as "[(Hloc&->&Hpending)|[(->&Hpending)|(Hloc&->&#Hshot)]]".
+  - (* In this case, the CmpXchg will succeed *)
+    wp_cmpxchg_suc.
+    (* This is how we close the invariant. We need "Hpending" and "Hflag" to go back into it *)
+    iMod ("Hclose" with "[$Hflag Hpending]") as "_".
+    { iNext. iRight. iLeft. iFrame "Hpending". done. }
+    iModIntro.
+    (* TODO: Now we increment by 2. *)
+
+    (* Now we did the incrementing, we need to open the invariant again to update the flag. *)
+    iInv "Hinv" as ">(%f&Hflag&Hcases)" "Hclose".
+    iDestruct "Hcases" as "[(Hc&_)|[(->&Hpending)|(Hc&_)]]".
+    1: { iExFalso.
+        (* TODO: This is contradictory. Use `pointsto_ne` and `iPoseProof` *) }
+    2: { (* TODO like case 1*) }
+    (* TODO: Update the flag. *)
+    
+    (* The key part. Update to `Shot` *)
+    iMod (shoot_upd with "Hpending") as "#Hshot".
+    (* And now, we can close the invariant again. Then, we are done. *)
+    iMod ("Hclose" with "[$Hflag Hloc]") as "_".
+    { iNext. 
+      (* TODO: close the invariant. Hint: We are now in the third case. *) }
+    iModIntro. done.
+  - wp_cmpxchg_fail. 1: done.
+    iMod ("Hclose" with "[$Hflag Hpending]") as "_".
+    (* This closes the invariant. Perhaps take inspiration here for some other todos :) *)
+    { iNext. iRight. iLeft. iFrame "Hpending". done. }
+    iModIntro.
+    do 8 wp_pure _.
+    do 2 wp_pure _.
+    wp_pure _.
+    (* Magic: we loop again. But since it is OK to loop forever, we can prove this case. The details go beyond this tutorial. *)
+    iApply "IH".
+  - wp_cmpxchg_fail. 1: done.
+    iMod ("Hclose" with "[$Hflag Hloc]") as "_".
+    { iNext. (* TODO: close the invariant again. *) }
+    iModIntro.
+    (* TODO: We are actually done here, since we know we are already "Shot". So there is nothing really left to do.*)
+Qed.
 
 Definition main : expr :=
   let: "flag" := ref #flag_before_update in
   let: "x" := ref #2 in
-  (thread_body "flag" "x" #() ||| 
-    thread_body "flag" "x" #()) ;;
+  (thread_body "flag" "x" |||
+    thread_body "flag" "x") ;;
   ! "x".
 
 Lemma threads :
   ⊢ WP main {{ v, ⌜v = #4⌝ }}.
-Admitted.
+Proof.
+  unfold main.
+  (* TODO: allocate the initial data *)
+  
+  (* Let's allocate the one-shot ghost state, and the invariant *)
+  iMod shoot_init as "(%γ&Hpending)".
+  iMod (inv_alloc nroot _ (flag_invariant γ flag loc) with "[$Hflag Hloc Hpending]") as "#Hinv".
+  { iNext. iLeft. iFrame "Hloc Hpending". done. }
+  wp_bind (par _ _).
+  iApply wp_par.
+  (* Now we handle both threads *)
+  { (* TODO: Use the `thread_helper` lemma from above. *) }
+  { (* TODO: The other thread. Same proof as the first. *) }
+  simpl.
+  (* Sometimes, we care about what our threads produce (v1 and v2). Here we do not. *)
+  iIntros (v1 v2) "(Hshot&_)".
+  iNext. wp_pures.
+  (* Open the invariant again. We should now be in the third state. *)
+  iInv "Hinv" as ">(%f&Hflag&Hcases)" "Hclose".
+  iDestruct "Hcases" as "[(Hloc&->&Hpending)|[(->&Hpending)|(Hloc&->&#Hshot2)]]".
+  { iExFalso. (* TODO: This case is impossible. Use `shot_not_pending` *) }
+  { iExFalso. (* TODO: as above *) }
+  (* TODO: do the load *)
+  
+  (* Let's close the invariant again. *)
+  iMod ("Hclose" with "[$Hflag Hshot Hloc]") as "_".
+  { iNext. (* TODO: Which case are we in again? *) }
+  (* And then, we are actually _done_ *)
+  done.
+Qed.
 
 End parallelism.
